Partially revert previous revert, as it reverted some good changes.
This partially reverts commit fa38a24583e984035b0b71c74d7e1a054b280412.
It also makes some further changes.

The definition of the Inductive Proof is not reverted because the
notation needs to be made available first.

src/FirstOrderLogic.v
@@ -16,6 +16,8 @@ Implicit Types (type : types) (context arity : list types).
 
 Section Syntax.
 
+(* Coq does not generate useful schemes for this nested inductive type.
+   We mostly just use fix and match instead. *)
 Section TermDef. #[local] Unset Elimination Schemes.
 Inductive Term context | : types -> Type :=
 | var (ind : ListIndex context) : Term (ListIndex.ref context ind)
@@ -23,8 +25,8 @@ Inductive Term context | : types -> Type :=
                     (args : Heterolist Term arity) : Term type.
 End TermDef.
 
-Section var'. Context {context type} (occ : Occ type context).
-Import (notations) EqNotations.
+Section var'. Import (notations) EqNotations.
+Context {context type} (occ : Occ type context).
 Definition var' : Term context type :=
 rew [Term context] Occ.ref_toIndex occ in var (Occ.toIndex occ).
 End var'.
@@ -87,7 +89,7 @@ Definition neg {context} (formula : Formula context)
   : Formula context :=
 impl formula contradiction.
 
-Definition exist {type context} (formula : Formula (type :: context))
+Definition exist {context type} (formula : Formula (type :: context))
   : Formula context :=
 neg (univ (neg formula)).
 
@@ -106,8 +108,10 @@ Fixpoint addContext [type] (term : Term context type)
 end.
 End addContext.
 
-(* Constructing `Value`s to use in substitutions. *)
-Definition id_values {context} : Substitutions context context :=
+(* Constructing substitutions. *)
+
+(* Identity subsitution.  Has no effect. *)
+Definition id_subst {context} : Substitutions context context :=
 Heterolist.mapList context var.
 
 (* TODO generalise this to adding multiple types like addContext? *)
@@ -116,7 +120,7 @@ Heterolist.mapList context var.
    This is achieved by incrementing the de Bruijn indexes of the terms
    to substitute (achieved by `Heterolist.map (addContext [type])`) and
    adding an identity substitution at the front (achieved by
-   `var' Occ_head ::`). *)
+   `var ListIndex.head ::`). *)
 Definition add1ContextToSubst {type context context'}
   (values : Substitutions context context')
   : Substitutions (type :: context) (type :: context') :=
@@ -124,10 +128,11 @@ var ListIndex.head :: Heterolist.map (addContext [type]) values.
 
 
 Lemma addContext_to_id_subst {type context}
-  : add1ContextToSubst id_values = @id_values (type :: context).
-unfold add1ContextToSubst, id_values at 2; simpl; f_equal.
+  : add1ContextToSubst id_subst = @id_subst (type :: context).
+unfold add1ContextToSubst, id_subst at 2; simpl; f_equal.
 apply Heterolist.map_mapList.
 Qed.
+
 
 Section TermSubst.
 Context {context context'} (values : Substitutions context context').
@@ -229,7 +234,13 @@ Section Proofs.
 Section defs.
 
 (* Note: experimental. *)
-Notation Assumptions context := (Formula context -> Type) (only parsing).
+Notation Assumptions context := (list (Formula context)) (only parsing).
+Notation "↑[ type ] assumptions" :=
+  (List.map (formula_subst (Heterolist.map (addContext [type]) id_subst))
+            assumptions)
+    (at level 8, right associativity).
+Notation "↑ assumptions" := (↑[_] assumptions)
+    (at level 8, right associativity).
 
 (* We define proofs in a context of free variables, with a set of
    assumptions that is allowed to refer to the variables. So proofs of
@@ -258,20 +269,28 @@ Module FOLFormulaNotations.
   Open Scope first_order_formula.
 
   Notation "⊥" := contradiction : first_order_formula.
-  Infix "->'" := impl (at level 60, right associativity) : first_order_formula.
+  Infix "→" := impl
+      (at level 60, right associativity) : first_order_formula.
 
-  Notation "¬ φ" := (neg φ) (at level 35, right associativity)
-    : first_order_formula.
+  Notation "¬ φ" := (neg φ)
+      (at level 35, right associativity) : first_order_formula.
 
-  Notation "∀' φ" := (univ φ) (at level 70, right associativity).
-  Notation "∃' φ" := (exist φ) (at level 70, right associativity).
+  Notation "∀'[ type ] φ" := (univ (type := type) φ)
+      (at level 70, right associativity) : first_order_formula.
+  Notation "∀' φ" := (univ φ)
+      (at level 70, right associativity) : first_order_formula.
+  Notation "∃'[ type ] φ" := (exist (type := type) φ)
+      (at level 70, right associativity) : first_order_formula.
+  Notation "∃' φ" := (exist φ)
+      (at level 70, right associativity) : first_order_formula.
 
+  (* Test the notation *)
   (* Example: given a predicate symbol `formula` with one argument, the
      formula `∃ x, ¬(formula x)`. *)
-  Check fun formula => ∃' ¬predApp' formula [var' Occ_head].
+  Check fun formula => ∃' ¬predApp' formula [var ListIndex.head].
   (* or more generally, given a formula with one free variable, applying
      it by substitution instead. *)
-  Check fun formula => ∃' ¬formula_subst [var' Occ_head] formula.
+  Check fun formula => ∃' ¬formula_subst [var ListIndex.head] formula.
 End FOLFormulaNotations.
 
 
@@ -309,7 +328,7 @@ Import (notations) FOLFormulaNotations.
 
 Succeed Check eq_refl :
 mysentence = ∀' predApp eq_n (var head) (app zero)
-                ->' ¬predApp eq_n (var head) (app succ (app zero)).
+                → ¬predApp eq_n (var head) (app succ (app zero)).
 
 (* The expression could be in any context starting with
    `[bool'; nat'; nat'; ...]`. We need to specify the type only so that
@@ -322,8 +341,8 @@ Let sampleFormula : Formula [_; _; _]%list :=
 let x := var (fromTail (fromTail head)) in
 let y := var (fromTail head) in
 let b := var head in
-(predApp eq_b (app leq x y) b) ->' (predApp eq_b (app leq y x) b)
-                               ->' (predApp eq_n x y).
+(predApp eq_b (app leq x y) b) → (predApp eq_b (app leq y x) b)
+                               → (predApp eq_n x y).
 
 (* TODO: find and put implementation of actual Nat.leqb here *)
 Fixpoint leqb (m n : nat) : bool := match m, n with
